refactor ChordProof.v into multiple files

systems/ChordProof.v
@@ -2,12 +2,12 @@ Require Import StructTact.StructTactics.
 Require Import StructTact.Util.
 Require Import Verdi.DynamicNet.
 Require Import Verdi.Chord.
+Require Import Arith.
+Require Import Verdi.ChordProps.
 Require Coqlib.
 Require Import List.
 Import ListNotations.
-Require Import Arith.
 Require Import mathcomp.ssreflect.ssreflect.
-Require Import Omega.
 
 Set Bullet Behavior "Strict Subproofs".
 
@@ -53,58 +53,6 @@ Section ChordProof.
   Notation e_recv := (e_recv addr payload timeout).
   Notation e_timeout := (e_timeout addr payload timeout).
   Notation e_fail := (e_fail addr payload timeout).
-
-  Inductive between : id -> id -> id -> Prop :=
-  | BetweenMono :
-      forall a x b, a < b -> a < x -> x < b -> between a x b
-  | BetweenWrapL :
-      forall a x b, a >= b -> a < x -> between a x b
-  | BetweenWrapR :
-      forall a x b, a >= b -> x < b -> between a x b.
-
-  Ltac inv_between :=
-    match goal with
-    | [H: between _ _ _ |- _] => inv H
-    end.
-
-  Lemma between_between_bool_equiv :
-    forall a x b,
-      between a x b <-> between_bool a x b = true.
-  Proof.
-    unfold between_bool.
-    intros.
-    split; intros.
-    - inv_between;
-        repeat break_if;
-        omega || reflexivity.
-    - repeat break_if;
-        constructor;
-        congruence || omega.
-  Qed.
-
-  Lemma between_bool_true_between :
-    forall a x b,
-      between_bool a x b = true ->
-      between a x b.
-  Proof.
-    intros.
-    now rewrite between_between_bool_equiv.
-  Qed.
-
-  Lemma between_bool_false_not_between :
-    forall a x b,
-      between_bool a x b = false ->
-      ~ between a x b.
-  Proof.
-    intros.
-    rewrite between_between_bool_equiv; congruence.
-  Qed.
-
-  Inductive request_response_pair : payload -> payload -> Prop :=
-  | pair_GetBestPredecessor : forall n p, request_response_pair (GetBestPredecessor n) (GotBestPredecessor p)
-  | pair_GetSuccList : forall l, request_response_pair GetSuccList (GotSuccList l)
-  | pair_GetPredAndSuccs : forall p l, request_response_pair GetPredAndSuccs (GotPredAndSuccs p l)
-  | pair_Ping : request_response_pair Ping Pong.
 
   Inductive timeout_constraint : global_state -> addr -> timeout -> Prop :=
   | Tick_unconstrained : forall gst h,
@@ -202,35 +150,6 @@ Section ChordProof.
 
   Notation step_dynamic := (step_dynamic addr addr_eq_dec payload data timeout timeout_eq_dec start_handler recv_handler timeout_handler timeout_constraint failure_constraint).
 
-  Inductive request_payload : payload -> Prop :=
-  | req_GetBestPredecessor : forall p, request_payload (GetBestPredecessor p)
-  | req_GetSuccList : request_payload GetSuccList
-  | req_GetPredAndSuccs : request_payload GetPredAndSuccs
-  | req_Ping : request_payload Ping.
-
-  Inductive response_payload : payload -> Prop :=
-  | res_GotBestPredecessor : forall p, response_payload (GotBestPredecessor p)
-  | res_GotSuccList : forall l, response_payload (GotSuccList l)
-  | res_GotPredAndSuccs : forall p l, response_payload (GotPredAndSuccs p l)
-  | res_Pong : response_payload Pong
-  | res_Busy : response_payload Busy.
-
-  Ltac request_payload_inversion :=
-    match goal with
-      | H : request_payload _ |- _ => inv H
-    end.
-
-  Lemma is_request_same_as_request_payload : forall msg : payload,
-      is_request msg = true <-> request_payload msg.
-  Proof.
-    unfold is_request.
-    intuition.
-    - break_match;
-        discriminate ||
-        eauto using req_GetBestPredecessor, req_GetSuccList, req_GetPredAndSuccs, req_Ping.
-    - now request_payload_inversion.
-  Qed.
-
   Lemma busy_response_exists :
     forall msg st' sends nts cts src dst st,
       request_payload msg ->
@@ -242,16 +161,6 @@ Section ChordProof.
     break_if;
     tuple_inversion;
     now apply in_eq.
-  Qed.
-
-  Lemma safe_msgs :
-    forall msg,
-      is_safe msg = true ->
-      msg = Ping \/ msg = Notify.
-  Proof.
-    unfold is_safe.
-    intuition.
-    break_match; auto || discriminate.
   Qed.
 
   Lemma unsafe_msgs_not_safe_ones :
