systems/ChordDefinitionLemmas.v
@@ -1,0 +1,350 @@
+Require Import List.
+Import ListNotations.
+
+Require Import StructTact.StructTactics.
+Require Import Verdi.Chord.
+Require Import Verdi.ChordProps.
+
+Section ChordDefinitionLemmas.
+  Variable SUCC_LIST_LEN : nat.
+  Variable N : nat.
+  Variable hash : addr -> id.
+  Notation start_handler := (start_handler SUCC_LIST_LEN hash).
+  Notation recv_handler := (recv_handler SUCC_LIST_LEN hash).
+  Notation timeout_handler := (timeout_handler hash).
+  Notation tick_handler := (tick_handler hash).
+  Notation handle_query_res := (handle_query_res SUCC_LIST_LEN hash).
+  Notation handle_query_timeout := (handle_query_timeout hash).
+  Notation make_pointer := (make_pointer hash).
+  Notation end_query := (end_query hash).
+  Notation start_query := (start_query hash).
+  Notation handle_stabilize := (handle_stabilize SUCC_LIST_LEN hash).
+  Notation try_rectify := (try_rectify hash).
+  Notation make_succs := (make_succs SUCC_LIST_LEN).
+
+
+  (* Definition lemmas *)
+  Lemma handle_query_req_busy_definition :
+    forall src dst st msg st' ms newts clearedts,
+      handle_query_req_busy src dst st msg = (st', ms, newts, clearedts) ->
+      st' = delay_query st src msg /\
+      ms = [(src, Busy)] /\
+      clearedts = [] /\
+      ((delayed_queries st = [] /\ newts = [KeepaliveTick]) \/
+       (delayed_queries st <> [] /\ newts = [])).
+  Proof.
+    unfold handle_query_req_busy.
+    intros.
+    repeat break_match; tuple_inversion; tauto.
+  Qed.
+
+  Lemma handle_query_res_definition :
+    forall src dst st blank q p st' ms newts clearedts,
+      handle_query_res src dst st blank q p = (st', ms, newts, clearedts) ->
+      (request_payload p /\
+       st' = delay_query st src p /\
+       clearedts = [] /\
+       (delayed_queries st = [] /\
+        newts = [KeepaliveTick]) \/
+       (delayed_queries st <> [] /\
+        newts = [])) \/
+      (p = Busy /\
+       st' = st /\
+       newts = timeouts_in st /\
+       clearedts = timeouts_in st) \/
+      (exists n,
+          q = Rectify n /\
+          p = Pong /\
+          (exists pr,
+              pred st = Some pr /\
+              end_query dst (handle_rectify st pr n) = (st', ms, newts, clearedts)) \/
+          (pred st = None /\
+           end_query dst (update_pred st n, [], [], []) = (st', ms, newts, clearedts))) \/
+      (q = Stabilize /\
+       (exists new_succ succs,
+           p = GotPredAndSuccs (Some new_succ) succs /\
+           handle_stabilize dst (make_pointer src) st q new_succ succs = (st', ms, newts, clearedts)) \/
+       (exists succs,
+           p = GotPredAndSuccs None succs /\
+           end_query dst (st, [], [], []) = (st', ms, newts, clearedts))) \/
+      (exists new_succ,
+          q = Stabilize2 new_succ /\
+          exists succs,
+            p = GotSuccList succs /\
+            end_query dst (update_succ_list st (make_succs new_succ succs),
+                           [(addr_of new_succ, Notify)], [], []) = (st', ms, newts, clearedts)) \/
+      (exists k,
+          q = Join k /\
+          (exists bestpred,
+              p = GotBestPredecessor bestpred /\
+              clearedts = [Request src (GetBestPredecessor (make_pointer dst))] /\
+              st' = st /\
+              (addr_of bestpred = src /\
+               ms = [(src, GetSuccList)] /\
+               newts = [Request src GetSuccList]) \/
+              (addr_of bestpred <> src /\
+               ms = [(addr_of bestpred, (GetBestPredecessor (make_pointer dst)))] /\
+               newts = [Request (addr_of bestpred) (GetBestPredecessor (make_pointer dst))])) \/
+          (p = GotSuccList [] /\
+           end_query dst (st, [], [], []) = (st', ms, newts, clearedts)) \/
+          (exists new_succ rest,
+              p = GotSuccList (new_succ :: rest) /\
+              start_query (addr_of new_succ) st (Join2 new_succ) = (st', ms, newts, clearedts))) \/
+      (exists new_succ succs,
+          q = Join2 new_succ /\
+          p = GotSuccList succs /\
+          add_tick (end_query dst (update_for_join st (make_succs new_succ succs), [], [], [])) = (st', ms, newts, clearedts)) \/
+      st' = st /\ ms = [] /\ newts = [] /\ clearedts = [].
+  Proof.
+    unfold handle_query_res.
+    intros.
+    repeat break_match; try tuple_inversion; try tauto.
+    - right. right. left. eexists. intuition eauto.
+    - intuition eauto.
+    - intuition eauto.
+    - intuition eauto.
+    - intuition eauto.
+    - do 5 right. left.
+      exists p0. left. firstorder.
+      eexists; intuition eauto.
+    - do 5 right. left.
+      exists p0. intuition eauto.
+    - repeat find_rewrite.
+      do 5 right. left.
+      exists p0. right.
+      intuition.
+    - do 5 right. left.
+      exists p0.
+      intuition eauto.
+    - intuition eauto.
+  Qed.
+
+  Lemma recv_handler_definition :
+    forall src dst st p st' ms newts clearedts,
+      recv_handler src dst st p = (st', ms, newts, clearedts) ->
+      p = Ping /\
+      st' = st /\
+      ms = [(src, Pong)] /\
+      newts = [] /\
+      clearedts = [] \/
+
+      p = Notify /\
+      st' = set_rectify_with st (make_pointer src) /\
+      ms = [] /\
+      newts = [] /\
+      clearedts = [] \/
+
+      (exists qd q qm,
+          cur_request st = Some (qd, q, qm) /\
+          (request_payload p /\
+           st' = delay_query st src p /\
+           clearedts = [] /\
+           (delayed_queries st = [] /\
+            newts = [KeepaliveTick]) \/
+           (delayed_queries st <> [] /\
+            newts = [])) \/
+          (p = Busy /\
+           st' = st /\
+           newts = timeouts_in st /\
+           clearedts = timeouts_in st) \/
+          (exists n,
+              q = Rectify n /\
+              p = Pong /\
+              (exists pr,
+              pred st = Some pr /\
+              end_query dst (handle_rectify st pr n) = (st', ms, newts, clearedts)) \/
+          (pred st = None /\
+           end_query dst (update_pred st n, [], [], []) = (st', ms, newts, clearedts))) \/
+      (q = Stabilize /\
+       (exists new_succ succs,
+           p = GotPredAndSuccs (Some new_succ) succs /\
+           handle_stabilize dst (make_pointer src) st q new_succ succs = (st', ms, newts, clearedts)) \/
+       (exists succs,
+           p = GotPredAndSuccs None succs /\
+           end_query dst (st, [], [], []) = (st', ms, newts, clearedts))) \/
+      (exists new_succ,
+          q = Stabilize2 new_succ /\
+          exists succs,
+            p = GotSuccList succs /\
+            end_query dst (update_succ_list st (make_succs new_succ succs),
+                           [(addr_of new_succ, Notify)], [], []) = (st', ms, newts, clearedts)) \/
+      (exists k,
+          q = Join k /\
+          (exists bestpred,
+              p = GotBestPredecessor bestpred /\
+              clearedts = [Request src (GetBestPredecessor (make_pointer dst))] /\
+              st' = st /\
+              (addr_of bestpred = src /\
+               ms = [(src, GetSuccList)] /\
+               newts = [Request src GetSuccList]) \/
+              (addr_of bestpred <> src /\
+               ms = [(addr_of bestpred, (GetBestPredecessor (make_pointer dst)))] /\
+               newts = [Request (addr_of bestpred) (GetBestPredecessor (make_pointer dst))])) \/
+          (p = GotSuccList [] /\
+           end_query dst (st, [], [], []) = (st', ms, newts, clearedts)) \/
+          (exists new_succ rest,
+              p = GotSuccList (new_succ :: rest) /\
+              start_query (addr_of new_succ) st (Join2 new_succ) = (st', ms, newts, clearedts))) \/
+      (exists new_succ succs,
+          q = Join2 new_succ /\
+          p = GotSuccList succs /\
+          add_tick (end_query dst (update_for_join st (make_succs new_succ succs), [], [], [])) = (st', ms, newts, clearedts)) \/
+      st' = st /\ ms = [] /\ newts = [] /\ clearedts = []
+      ) \/
+
+      (cur_request st = None /\
+       st' = st /\
+       clearedts = [] /\
+       newts = [] /\
+       ((exists h,
+           p = GetBestPredecessor h /\
+           ms = [(src, GotBestPredecessor (best_predecessor (ptr st) (succ_list st) (id_of h)))]) \/
+       (p = GetSuccList /\
+        ms = [(src, GotSuccList (succ_list st))]) \/
+       (p = GetPredAndSuccs /\
+        ms = [(src, GotPredAndSuccs (pred st) (succ_list st))]))) \/
+
+      st = st' /\ ms = [] /\ newts = [] /\ clearedts = [].
+  Proof.
+    unfold recv_handler.
+    intros.
+    break_if.
+    - unfold handle_safe_msg, handle_notify in *.
+      find_apply_lem_hyp safe_msgs; break_or_hyp;
+      tuple_inversion; intuition.
+    - repeat break_match.
+      + find_eapply_lem_hyp handle_query_req_busy_definition.
+        repeat break_and.
+        find_apply_lem_hyp is_request_same_as_request_payload.
+        do 2 right. left.
+        repeat eexists; left; split; eauto.
+        repeat split.
+        repeat break_and.
+        break_or_hyp; intuition eauto.
+      + find_eapply_lem_hyp handle_query_res_definition.
+        do 2 right. left.
+        repeat eexists; intuition eauto.
+      + unfold handle_query_req in *.
+        break_match;
+          try discriminate;
+          repeat find_inversion;
+          try tuple_inversion;
+          intuition eauto.
+      + tuple_inversion; intuition eauto.
+      + tuple_inversion; intuition eauto.
+  Qed.
+
+  Lemma try_rectify_definition :
+    forall h st ms nts cts st' ms' nts' cts',
+      try_rectify h (st, ms, nts, cts) = (st', ms', nts', cts') ->
+      (joined st = true /\
+       (exists new,
+           rectify_with st = Some new /\
+           (exists x sq_ms sq_nts sq_cts,
+               pred st = Some x /\
+               start_query h (clear_rectify_with st) (Rectify new) = (st', sq_ms, sq_nts, sq_cts) /\
+               ms' = ms ++ sq_ms /\
+               nts' = nts ++ sq_nts /\
+               cts' = cts ++ sq_cts) \/
+           (pred st = None /\
+            st' = clear_rectify_with (update_pred st new) /\
+            ms' = ms /\
+            nts' = nts /\
+            cts' = cts))) \/
+      ((joined st = false \/ rectify_with st = None) /\
+       (st', ms', nts', cts') = (st, ms, nts, cts)).
+  Proof.
+    unfold try_rectify.
+    intros.
+    repeat break_match; tuple_inversion.
+    - left.
+      split; eauto.
+      intuition eauto.
+      exists p.
+      left.
+      intuition eauto.
+      repeat eexists; intuition eauto.
+    - left.
+      split; try tauto.
+      eexists; right; split; eauto.
+    - tauto.
+    - tauto.
+  Qed.
+
+  Lemma start_query_definition : 
+    forall h st k st' ms nts cts,
+      start_query h st k = (st', ms, nts, cts) ->
+      (exists dst msg,
+          make_request hash h st k = Some (dst, msg) /\
+          st' = update_query st dst k msg /\
+          ms = [(addr_of dst, msg)] /\
+          nts = [Request (addr_of dst) msg] /\
+          cts = timeouts_in st) \/
+      (make_request hash h st k = None /\
+       st' = st /\
+       ms = [] /\
+       ms = [] /\
+       nts = [] /\
+       cts = []).
+  Proof.
+    unfold start_query.
+    intros.
+    repeat break_match; tuple_inversion; try tauto.
+    left; repeat eexists.
+  Qed.
+
+  Lemma handle_delayed_queries_definition :
+    forall h st st' ms nts cts,
+     handle_delayed_queries h st = (st', ms, nts, cts) ->
+     st' = clear_delayed_queries st /\
+     ms = concat (map (handle_delayed_query h st) (delayed_queries st)) /\
+     nts = [] /\
+     cts = [KeepaliveTick].
+  Proof.
+    unfold handle_delayed_queries.
+    intros.
+    tuple_inversion.
+    intuition eauto.
+  Qed.
+
+  Lemma end_query_definition :
+    forall h st ms newts clearedts st' ms' newts' clearedts',
+      end_query h (st, ms, newts, clearedts) = (st', ms', newts', clearedts') ->
+      exists st'' ms'',
+        handle_delayed_queries h (clear_query st) = (st'', ms'', [], [KeepaliveTick]) /\
+        try_rectify h (st'', ms'' ++ ms, newts, timeouts_in st ++ [KeepaliveTick] ++ clearedts) = (st', ms', newts', clearedts').
+  Proof.
+    unfold end_query.
+    intros.
+    repeat break_let.
+    find_apply_lem_hyp handle_delayed_queries_definition.
+    repeat (break_and || break_or_hyp || break_exists).
+    subst_max.
+    repeat eexists; eauto.
+  Qed.
+
+  Lemma handle_rectify_definition :
+    forall st my_pred notifier st' ms nts cts,
+      handle_rectify st my_pred notifier = (st', ms, nts, cts) ->
+      ms = [] /\
+      nts = [] /\
+      cts = [] /\
+      (between (id_of my_pred) (id_of notifier) (id_of (ptr st)) /\
+       st' = update_pred st notifier \/
+       ~ between (id_of my_pred) (id_of notifier) (id_of (ptr st)) /\
+       st' = st).
+  Proof.
+    unfold handle_rectify.
+    intros.
+    rewrite between_between_bool_equiv.
+    break_if; tuple_inversion; firstorder.
+  Qed.
+
+  Ltac expand_def :=
+    repeat (try break_or_hyp; try break_and; try break_exists);
+    subst_max;
+    try tuple_inversion;
+    try (exfalso; tauto).
+
+End ChordDefinitionLemmas.
+
