systems/ChordProps.v
@@ -1,0 +1,121 @@
+Require Import Omega.
+
+Require Import Verdi.Chord.
+Require Import StructTact.StructTactics.
+
+(* Requests and responses *)
+Inductive request_payload : payload -> Prop :=
+| req_GetBestPredecessor : forall p, request_payload (GetBestPredecessor p)
+| req_GetSuccList : request_payload GetSuccList
+| req_GetPredAndSuccs : request_payload GetPredAndSuccs
+| req_Ping : request_payload Ping.
+
+Ltac request_payload_inversion :=
+  match goal with
+  | H : request_payload _ |- _ => inv H
+  end.
+
+Inductive response_payload : payload -> Prop :=
+| res_GotBestPredecessor : forall p, response_payload (GotBestPredecessor p)
+| res_GotSuccList : forall l, response_payload (GotSuccList l)
+| res_GotPredAndSuccs : forall p l, response_payload (GotPredAndSuccs p l)
+| res_Pong : response_payload Pong
+| res_Busy : response_payload Busy.
+
+Inductive request_response_pair : payload -> payload -> Prop :=
+| pair_GetBestPredecessor : forall n p, request_response_pair (GetBestPredecessor n) (GotBestPredecessor p)
+| pair_GetSuccList : forall l, request_response_pair GetSuccList (GotSuccList l)
+| pair_GetPredAndSuccs : forall p l, request_response_pair GetPredAndSuccs (GotPredAndSuccs p l)
+| pair_Ping : request_response_pair Ping Pong.
+
+Lemma is_request_same_as_request_payload : forall msg : payload,
+    is_request msg = true <-> request_payload msg.
+Proof.
+  unfold is_request.
+  intuition.
+  - break_match;
+    discriminate || eauto using req_GetBestPredecessor, req_GetSuccList, req_GetPredAndSuccs, req_Ping.
+  - now request_payload_inversion.
+Qed.
+
+(* Safe messages (Notify and Ping) *)
+Lemma safe_msgs :
+  forall msg,
+    is_safe msg = true ->
+    msg = Ping \/ msg = Notify.
+Proof.
+  unfold is_safe.
+  intuition.
+  break_match; auto || discriminate.
+Qed.
+
+Lemma only_safe_request_is_Ping :
+  forall msg,
+    request_payload msg ->
+    is_safe msg = true ->
+    msg = Ping.
+Proof.
+  intuition.
+  request_payload_inversion;
+    find_apply_lem_hyp safe_msgs;
+    break_or_hyp;
+    auto || discriminate.
+Qed.
+
+(* between_bool from Chord.v but in Prop *)
+Inductive between : id -> id -> id -> Prop :=
+| BetweenMono :
+    forall a x b, a < b -> a < x -> x < b -> between a x b
+| BetweenWrapL :
+    forall a x b, a >= b -> a < x -> between a x b
+| BetweenWrapR :
+    forall a x b, a >= b -> x < b -> between a x b.
+
+Ltac inv_between :=
+  match goal with
+  | [H: between _ _ _ |- _] => inv H
+  end.
+
+Lemma between_between_bool_equiv :
+  forall a x b,
+    between a x b <-> between_bool a x b = true.
+Proof.
+  unfold between_bool.
+  intros.
+  split; intros.
+  - inv_between;
+    repeat break_if;
+    omega || reflexivity.
+  - repeat break_if;
+    constructor;
+    congruence || omega.
+Qed.
+
+Lemma between_bool_true_between :
+  forall a x b,
+    between_bool a x b = true ->
+    between a x b.
+Proof.
+  intros.
+  now rewrite between_between_bool_equiv.
+Qed.
+
+Lemma between_bool_false_not_between :
+  forall a x b,
+    between_bool a x b = false ->
+    ~ between a x b.
+Proof.
+  intros.
+  rewrite between_between_bool_equiv; congruence.
+Qed.
+
+Lemma unsafe_msgs_not_safe_ones :
+  forall msg,
+    is_safe msg = false ->
+    msg <> Notify /\ msg <> Ping.
+Proof.
+  unfold is_safe.
+  intuition;
+    break_match;
+    easy.
+Qed.
